ContextBasicDenotation/theories/TermOpen.v
@@ -293,6 +293,59 @@ Proof.
 	            (open_tm (d + 3 + k) (vfvar y) e))
 	      end.
 	      apply H1; set_solver.
+	  - f_equal.
+	    + match goal with
+	      | |- lstore_instantiate_value_split_at d _ _ ?v =
+	           lstore_instantiate_value_split_at d _ _
+	             (open_value (d + k) (vfvar y) ?v) =>
+	          change (lstore_instantiate_value_at d
+	            (lstore_swap (LVBound k) (LVFree y) σ) v =
+	          lstore_instantiate_value_at d σ
+	            (open_value (d + k) (vfvar y) v))
+	      end.
+	      apply H; set_solver.
+	    + match goal with
+	      | |- lstore_instantiate_value_split_at d _ _ ?v =
+	           lstore_instantiate_value_split_at d _ _
+	             (open_value (d + k) (vfvar y) ?v) =>
+	          change (lstore_instantiate_value_at d
+	            (lstore_swap (LVBound k) (LVFree y) σ) v =
+	          lstore_instantiate_value_at d σ
+	            (open_value (d + k) (vfvar y) v))
+	      end.
+	      apply H0; set_solver.
+	  - f_equal.
+	    + match goal with
+	      | |- lstore_instantiate_value_split_at d _ _ ?v =
+	           lstore_instantiate_value_split_at d _ _
+	             (open_value (d + k) (vfvar y) ?v) =>
+	          change (lstore_instantiate_value_at d
+	            (lstore_swap (LVBound k) (LVFree y) σ) v =
+	          lstore_instantiate_value_at d σ
+	            (open_value (d + k) (vfvar y) v))
+	      end.
+	      apply H; set_solver.
+	    + match goal with
+	      | |- lstore_instantiate_tm_split_at d _ _ ?e =
+	           lstore_instantiate_tm_split_at d _ _
+	             (open_tm (d + k) (vfvar y) ?e) =>
+	          change (lstore_instantiate_tm_at d
+	            (lstore_swap (LVBound k) (LVFree y) σ) e =
+	          lstore_instantiate_tm_at d σ
+	            (open_tm (d + k) (vfvar y) e))
+	      end.
+	      apply H0; set_solver.
+	    + replace (d + k + 2) with (d + 2 + k) by lia.
+	      match goal with
+	      | |- lstore_instantiate_tm_split_at (d + 2) _ _ ?e =
+	           lstore_instantiate_tm_split_at (d + 2) _ _
+	             (open_tm (d + 2 + k) (vfvar y) ?e) =>
+	          change (lstore_instantiate_tm_at (d + 2)
+	            (lstore_swap (LVBound k) (LVFree y) σ) e =
+	          lstore_instantiate_tm_at (d + 2) σ
+	            (open_tm (d + 2 + k) (vfvar y) e))
+	      end.
+	      apply H1; set_solver.
 Qed.
 
 Lemma lstore_instantiate_tm_insert_open
