ContextBasicDenotation/theories/TermSyntax.v
@@ -43,8 +43,10 @@ Proof.
   - rewrite lvars_fv_union, H, H0. reflexivity.
   - apply H.
   - rewrite lvars_fv_union, H, H0. reflexivity.
-  - rewrite !lvars_fv_union, H, H0, H1. set_solver.
-  - rewrite !lvars_fv_union, H, H0, H1. set_solver.
+	  - rewrite !lvars_fv_union, H, H0, H1. set_solver.
+	  - rewrite !lvars_fv_union, H, H0, H1. set_solver.
+	  - rewrite !lvars_fv_union, H, H0, H1. set_solver.
+  - rewrite lvars_fv_union, H, H0. reflexivity.
   - rewrite !lvars_fv_union, H, H0, H1. set_solver.
 Qed.
 
@@ -114,6 +116,10 @@ Proof.
   - rewrite !lvars_at_depth_union, H, H0, H1. reflexivity.
   - rewrite !lvars_at_depth_union, H, H0, H1.
     replace (c + 3 + d) with (c + d + 3) by lia.
+    reflexivity.
+  - rewrite lvars_at_depth_union, H, H0. reflexivity.
+  - rewrite !lvars_at_depth_union, H, H0, H1.
+    replace (c + 2 + d) with (c + d + 2) by lia.
     reflexivity.
 Qed.
 
@@ -198,6 +204,14 @@ Proof.
     replace (d + k + 3) with (d + 3 + k) by lia.
     rewrite H1 by (rewrite ?lvars_fv_union in *; set_solver).
     rewrite <- !set_swap_union. set_solver.
+  - rewrite H by (rewrite ?lvars_fv_union in *; set_solver).
+    rewrite H0 by (rewrite ?lvars_fv_union in *; set_solver).
+    rewrite <- set_swap_union. reflexivity.
+  - rewrite H by (rewrite ?lvars_fv_union in *; set_solver).
+    rewrite H0 by (rewrite ?lvars_fv_union in *; set_solver).
+    replace (d + k + 2) with (d + 2 + k) by lia.
+    rewrite H1 by (rewrite ?lvars_fv_union in *; set_solver).
+    rewrite <- !set_swap_union. set_solver.
 Qed.
 
 Lemma value_lvars_at_open v d k y :
@@ -261,6 +275,41 @@ Proof.
   set_solver.
 Qed.
 
+Lemma lvars_bv_at_depth2_empty_of_open01 hd tl D :
+  lvars_bv (lvars_open 1 tl (lvars_open 0 hd D)) = ∅ ->
+  lvars_bv (lvars_at_depth 2 D) = ∅.
+Proof.
+  intros Hopen.
+  apply set_eq. intros k.
+  rewrite elem_of_empty.
+  split; [|set_solver].
+  intros Hk.
+  rewrite lvars_bv_elem in Hk.
+  apply lvars_at_depth_elem in Hk as [u [Hu Hdepth]].
+  destruct u as [n|x]; cbn [logic_var_at_depth] in Hdepth; [|discriminate].
+  destruct (decide (2 <= n)) as [H2n|H2n]; [|discriminate].
+  inversion Hdepth. subst k.
+  assert (LVBound n ∈ lvars_open 1 tl (lvars_open 0 hd D)) as Hopened.
+  {
+    rewrite !elem_of_set_swap.
+    match goal with
+    | |- ?u ∈ D =>
+        replace u with (LVBound n) by
+          (unfold swap; repeat destruct decide; try discriminate;
+           try match goal with H : LVBound _ = LVBound _ |- _ =>
+             inversion H; lia
+           end; reflexivity)
+    end.
+    exact Hu.
+  }
+  assert (n ∈ lvars_bv (lvars_open 1 tl (lvars_open 0 hd D))) as Hn.
+  { rewrite lvars_bv_elem. exact Hopened. }
+  change (n ∈ lvars_bv
+    ((fun k x => set_swap (LVBound k) (LVFree x)) 1 tl
+      ((fun k x => set_swap (LVBound k) (LVFree x)) 0 hd D))) in Hn.
+  set_solver.
+Qed.
+
 Lemma value_tm_lvars_no_bv_of_lc_mutual :
   (forall v,
       lc_value v ->
@@ -282,7 +331,9 @@ Proof.
 	    (fun v1 v2 Hlc1 IH1 Hlc2 IH2 => _)
 	    (fun v et ef Hlcv IHv Hlcet IHet Hlcef IHef => _)
 	    (fun root left right Hlcroot IHroot Hlcleft IHleft Hlcright IHright => _)
-	    (fun v eleaf enode L Hlcv IHv Hlcleaf IHeleaf Hbody IHnode => _)).
+	    (fun v eleaf enode L Hlcv IHv Hlcleaf IHeleaf Hbody IHnode => _)
+	    (fun hd tl Hlchd IHhd Hlctl IHtl => _)
+	    (fun v enil econs L Hlcv IHv Hlcnil IHnil Hbody IHcons => _)).
   - cbn [value_lvars value_lvars_at]. reflexivity.
   - cbn [value_lvars value_lvars_at].
     apply lvars_bv_singleton_free_atom.
@@ -404,6 +455,44 @@ Proof.
     rewrite tm_lvars_depth in IHnode.
     change (tm_lvars_at (0 + 3) enode) with (tm_lvars_at 3 enode).
     rewrite IHnode. set_solver.
+  - cbn [value_lvars tm_lvars value_lvars_at tm_lvars_at].
+    change (value_lvars_at 0 hd) with (value_lvars hd).
+    change (value_lvars_at 0 tl) with (value_lvars tl).
+    rewrite lvars_bv_union, IHhd, IHtl. set_solver.
+  - cbn [value_lvars tm_lvars value_lvars_at tm_lvars_at].
+    change (value_lvars_at 0 v) with (value_lvars v).
+    change (tm_lvars_at 0 enil) with (tm_lvars enil).
+    rewrite !lvars_bv_union, IHv, IHnil.
+    pose (hd := fresh_for (L ∪ fv_tm econs)).
+    assert (HhdL : hd ∉ L) by
+      (subst hd; pose proof (fresh_for_not_in (L ∪ fv_tm econs)); set_solver).
+    assert (Hhdfv : hd ∉ fv_tm econs) by
+      (subst hd; pose proof (fresh_for_not_in (L ∪ fv_tm econs)); set_solver).
+    pose (tl := fresh_for (L ∪ fv_tm econs ∪ {[hd]})).
+    assert (HtlL : tl ∉ L) by
+      (subst tl; pose proof (fresh_for_not_in (L ∪ fv_tm econs ∪ {[hd]}));
+       set_solver).
+    assert (Htlfv : tl ∉ fv_tm econs) by
+      (subst tl; pose proof (fresh_for_not_in (L ∪ fv_tm econs ∪ {[hd]}));
+       set_solver).
+    assert (Htl_hd : tl <> hd) by
+      (subst tl; pose proof (fresh_for_not_in (L ∪ fv_tm econs ∪ {[hd]}));
+       set_solver).
+    assert (Htl_nested : tl ∉ L ∪ {[hd]}) by set_solver.
+    specialize (IHcons hd tl HhdL Htl_nested).
+    unfold open_list_cons_branch, open_list_cons_branch_value in IHcons.
+    rewrite tm_lvars_open in IHcons.
+    2: {
+      pose proof (open_fv_tm
+        (open_tm 0 (vfvar hd) econs) (vfvar tl) 1) as Hfv_tl.
+      pose proof (open_fv_tm econs (vfvar hd) 0) as Hfv_hd.
+      cbn [fv_value] in *. set_solver.
+    }
+    rewrite tm_lvars_open in IHcons by exact Hhdfv.
+    apply lvars_bv_at_depth2_empty_of_open01 in IHcons.
+    rewrite tm_lvars_depth in IHcons.
+    change (tm_lvars_at (0 + 2) econs) with (tm_lvars_at 2 econs).
+    rewrite IHcons. set_solver.
 Qed.
 
 Lemma value_lvars_no_bv_of_lc v :
@@ -651,6 +740,13 @@ Proof.
     + apply H. rewrite !lvars_bv_union in H2. set_solver.
     + apply H0. rewrite !lvars_bv_union in H2. set_solver.
     + apply H1. rewrite !lvars_bv_union in H2. set_solver.
+  - f_equal.
+    + apply H. rewrite lvars_bv_union in H1. set_solver.
+    + apply H0. rewrite lvars_bv_union in H1. set_solver.
+  - f_equal.
+    + apply H. rewrite !lvars_bv_union in H2. set_solver.
+    + apply H0. rewrite !lvars_bv_union in H2. set_solver.
+    + apply H1. rewrite !lvars_bv_union in H2. set_solver.
 Qed.
 
 Lemma open_tm_shift_no_bv d x e :
@@ -868,6 +964,13 @@ Proof.
     replace (S d + 3) with (S (d + 3)) by lia.
     rewrite (H1 (d + 3) (k + 3)) by lia.
     reflexivity.
+  - rewrite H by exact H1.
+    rewrite H0 by exact H1. reflexivity.
+  - rewrite (H d k H2).
+    rewrite (H0 d k H2).
+    replace (S d + 2) with (S (d + 2)) by lia.
+    rewrite (H1 (d + 2) (k + 2)) by lia.
+    reflexivity.
 Qed.
 
 Lemma value_lvars_at_shift_under v d k :
@@ -922,6 +1025,15 @@ Proof.
     rewrite tm_lvars_at_shift_under by lia.
     cbn [tm_lvars_at].
     rewrite !value_lvars_at_bound0_under. set_solver.
+  - rewrite !value_lvars_at_shift_under by lia.
+    cbn [tm_lvars_at].
+    rewrite !value_lvars_at_bound0_under. set_solver.
+  - rewrite value_lvars_at_shift_under by lia.
+    rewrite tm_lvars_at_shift_under by lia.
+    replace (S d + 2) with (S (d + 2)) by lia.
+    rewrite tm_lvars_at_shift_under by lia.
+    cbn [tm_lvars_at].
+    rewrite !value_lvars_at_bound0_under. set_solver.
 Qed.
 
 Lemma tm_lvars_at_tapp_shift0_bound0 e d :
@@ -972,11 +1084,18 @@ with lstore_instantiate_tm_split_at
 	      tnode (lstore_instantiate_value_split_at d σf σb root)
 	        (lstore_instantiate_value_split_at d σf σb lft)
 	        (lstore_instantiate_value_split_at d σf σb rgt)
-	  | tmatchtree v eleaf enode =>
-	      tmatchtree (lstore_instantiate_value_split_at d σf σb v)
-	        (lstore_instantiate_tm_split_at d σf σb eleaf)
-	        (lstore_instantiate_tm_split_at (d + 3) σf σb enode)
-	  end.
+		  | tmatchtree v eleaf enode =>
+		      tmatchtree (lstore_instantiate_value_split_at d σf σb v)
+		        (lstore_instantiate_tm_split_at d σf σb eleaf)
+		        (lstore_instantiate_tm_split_at (d + 3) σf σb enode)
+		  | tcons hd tl =>
+		      tcons (lstore_instantiate_value_split_at d σf σb hd)
+		        (lstore_instantiate_value_split_at d σf σb tl)
+		  | tmatchlist v enil econs =>
+		      tmatchlist (lstore_instantiate_value_split_at d σf σb v)
+		        (lstore_instantiate_tm_split_at d σf σb enil)
+		        (lstore_instantiate_tm_split_at (d + 2) σf σb econs)
+		  end.
 
 Definition lstore_instantiate_value_at
     (d : nat) (σ : LStoreT) (v : value) : value :=
@@ -1085,6 +1204,8 @@ Proof.
   - f_equal; [apply H | apply H0 | apply H1]; set_solver.
   - f_equal; [apply H | apply H0 | apply H1]; set_solver.
   - f_equal; [apply H | apply H0 | apply H1]; set_solver.
+  - f_equal; [apply H | apply H0]; set_solver.
+  - f_equal; [apply H | apply H0 | apply H1]; set_solver.
 Qed.
 
 Lemma lstore_instantiate_tm_at_restrict_lvars e d (σ : LStoreT) X :
@@ -1164,6 +1285,8 @@ Proof.
   - f_equal; [apply H | apply H0 | apply H1]; set_solver.
   - f_equal; [apply H | apply H0 | apply H1]; set_solver.
   - f_equal; [apply H | apply H0 | apply H1]; set_solver.
+  - f_equal; [apply H | apply H0]; set_solver.
+  - f_equal; [apply H | apply H0 | apply H1]; set_solver.
 Qed.
 
 Lemma lstore_instantiate_tm_split_restrict_fv d (σf : StoreT) σb e X :
@@ -1221,7 +1344,11 @@ Proof.
       [apply H | apply H0 | apply H1]; exact H2.
   - rewrite subst_map_tnode. repeat f_equal;
       [apply H | apply H0 | apply H1]; exact H2.
-  - rewrite subst_map_tmatchtree. repeat f_equal;
+	  - rewrite subst_map_tmatchtree. repeat f_equal;
+	      [apply H | apply H0 | apply H1]; exact H2.
+  - rewrite subst_map_tcons. repeat f_equal;
+      [apply H | apply H0]; exact H1.
+  - rewrite subst_map_tmatchlist. repeat f_equal;
       [apply H | apply H0 | apply H1]; exact H2.
 Qed.
 
@@ -1297,6 +1424,12 @@ Proof.
     + apply H; set_solver.
     + apply H0; set_solver.
     + replace (S d + 3) with (S (d + 3)) by lia.
+      apply H1; set_solver.
+  - f_equal; [apply H | apply H0]; set_solver.
+  - f_equal.
+    + apply H; set_solver.
+    + apply H0; set_solver.
+    + replace (S d + 2) with (S (d + 2)) by lia.
       apply H1; set_solver.
 Qed.
 
