CoreLang/theories/SyntaxNotation.v
@@ -40,6 +40,7 @@ Notation tyctx := (gmap atom ty).
 Notation "'𝔹'" := TBool : core_scope.
 Notation "'ℕ'" := TNat : core_scope.
 Notation "'Tree'" := TTree : core_scope.
+Notation "'List'" := TList : core_scope.
 Notation "T1 '→' T2" := (TArrow T1 T2)
   (at level 99, right associativity) : core_scope.
 Notation "T1 ⇒ T2" := (TArrow T1 T2)
@@ -56,6 +57,7 @@ Definition constant_to_uint (c : constant) : option Number.uint :=
   | cnat n => Some (Nat.to_num_uint n)
   | cbool _ => None
   | ctree _ => None
+  | clist _ => None
   end.
 
 Number Notation constant constant_of_uint constant_to_uint : core_scope.
@@ -64,6 +66,7 @@ Notation "'#' n" := (vbvar n)
   (at level 5, format "# n") : core_scope.
 
 Notation "'leaf'" := (ctree tr_leaf) (only printing) : core_scope.
+Notation "'nil'" := (clist []) (only printing) : core_scope.
 
 Notation "'λ:' T ',' e" := (vlam T e)
   (at level 100, T at level 200, e at level 200,
@@ -90,13 +93,23 @@ Notation "'if' v 'then' et 'else' ef" := (tmatch v et ef)
 
 Notation "'Leaf'" := (vconst (ctree tr_leaf))
   (at level 20, format "Leaf") : core_scope.
+Notation "'Nil'" := (vconst (clist []))
+  (at level 20, format "Nil") : core_scope.
 Notation "'Node' r l rr" := (tnode r l rr)
   (at level 30, r at level 30, l at level 30, rr at level 30,
    format "Node  r  l  rr") : core_scope.
+Notation "'Cons' hd tl" := (tcons hd tl)
+  (at level 30, hd at level 30, tl at level 30,
+   format "Cons  hd  tl") : core_scope.
 Notation "'matchTree' v 'with' 'Leaf' '=>' el '|' 'Node' '=>' en" :=
   (tmatchtree v el en)
   (at level 100, v at level 200, el at level 200, en at level 200,
    format "'[v' matchTree  v  with '/' Leaf  =>  el '/' |  Node  =>  en ']'")
+  : core_scope.
+Notation "'matchList' v 'with' 'Nil' '=>' en '|' 'Cons' '=>' ec" :=
+  (tmatchlist v en ec)
+  (at level 100, v at level 200, en at level 200, ec at level 200,
+   format "'[v' matchList  v  with '/' Nil  =>  en '/' |  Cons  =>  ec ']'")
   : core_scope.
 
 Notation "'iszero' v" := (tprim op_eq0 v)
